compiler/backend/passes/pure_nestedcaseScript.sml
@@ -1,0 +1,74 @@
+open HolKernel Parse boolLib bossLib;
+
+open listTheory
+open pure_cexpTheory
+
+val _ = new_theory "pure_nestedcase";
+
+Definition updlast_def[simp]:
+  updlast [] rep = rep ∧
+  updlast [h] rep = rep ∧
+  updlast (h1::h2::t) rep = h1 :: updlast (h2::t) rep
+End
+
+Theorem updlast_EQ_NIL[simp]:
+  ∀l rep. updlast l rep = [] ⇔ rep = [] ∧ LENGTH l < 2
+Proof recInduct updlast_ind >> rw[]
+QED
+
+Theorem LAST_updlast:
+  ∀l rep. rep ≠ [] ⇒ LAST (updlast l rep) = LAST rep
+Proof
+  recInduct updlast_ind >> rw[] >> gs[] >> simp[LAST_CONS_cond]
+QED
+
+Definition lift_uscore1_def:
+  (lift_uscore1 (NestedCase c texp tv pes) =
+   if pes = [] then NestedCase c texp tv pes
+   else
+     case LAST pes of
+       (p,e) => if p = cepatUScore then
+                  case dest_nestedcase e of
+                    SOME (texp', _, pes') =>
+                      (case dest_var texp' of
+                         SOME vnm =>
+                           if tv = vnm then
+                             NestedCase c texp tv (updlast pes pes')
+                           else NestedCase c texp tv pes
+                       | NONE => NestedCase c texp tv pes)
+                  | NONE => NestedCase c texp tv pes
+                else
+                  NestedCase c texp tv pes) ∧
+  (lift_uscore1 e = e)
+End
+
+case x@v of
+  C (p,y) =>
+  D (p2,y) =>
+
+  -->
+
+  case x of
+     C (v, y) => ....
+   | _ => case x of
+             D(p2,_)
+
+
+             --->
+
+             case x of
+               C(v1,..)
+               D(v1,..)
+
+Overload lift_uscore = “gencexp_recurse lift_uscore1”
+
+Theorem lift_uscore_thm =
+        gencexp_recurse_def
+          |> CONJUNCTS
+          |> map SPEC_ALL
+          |> map (Q.INST [‘f’ |-> ‘lift_uscore1’])
+          |> map GEN_ALL |> LIST_CONJ
+          |> SRULE [lift_uscore1_def, SF boolSimps.ETA_ss,
+                    listTheory.LAST_MAP]
+
+val _ = export_theory();
